strengthen lifetime logic: make lft_userN disjoint from lftN so it remains available during atomic accessors

theories/lifetime/lifetime_sig.v
@@ -6,9 +6,9 @@ From iris.bi Require Import fractional.
 Set Default Proof Using "Type".
 
 Definition lftN : namespace := nroot .@ "lft".
-(** A mask inside the lifetime logic namespace that users may use.
-This is still available in the "consequence" view shift of borrow accessors. *)
-Definition lft_userN : namespace := nroot .@ "lft" .@ "usr".
+(** A (disjoint) mask that is available in the "consequence" view shift of
+    borrow accessors. *)
+Definition lft_userN : namespace := nroot .@ "lft_usr".
 
 Module Type lifetime_sig.
   (** CMRAs needed by the lifetime logic  *)
@@ -96,7 +96,7 @@ Module Type lifetime_sig.
   Parameter lft_dead_static : [† static] -∗ False.
 
   Parameter lft_create : ∀ E, ↑lftN ⊆ E →
-    lft_ctx ={E}=∗ ∃ κ, 1.[κ] ∗ □ (1.[κ] ={↑lftN}[↑lft_userN]▷=∗ [†κ]).
+    lft_ctx ={E}=∗ ∃ κ, 1.[κ] ∗ □ (1.[κ] ={↑lftN ∪ ↑lft_userN}[↑lft_userN]▷=∗ [†κ]).
   Parameter bor_create : ∀ E κ P,
     ↑lftN ⊆ E → lft_ctx -∗ ▷ P ={E}=∗ &{κ} P ∗ ([†κ] ={E}=∗ ▷ P).
   Parameter bor_fake : ∀ E κ P,
