theories/typing/function.v
@@ -285,8 +285,8 @@ Section typing.
         iDestruct "Hϝ" as  (κ') "(EQ & Htk & _)". iDestruct "EQ" as %EQ.
         rewrite /= left_id in EQ. subst κ'. simpl. wp_rec. wp_bind Endlft.
         iSpecialize ("Hinh" with "Htk"). iClear "Hκs".
-        iApply (wp_mask_mono _ (↑lftN)); first done.
-        iApply (wp_step_fupd with "Hinh"); [solve_ndisj..|]. wp_seq.
+        iApply (wp_mask_mono _ (↑lftN ∪ ↑lft_userN)); first done.
+        iApply (wp_step_fupd with "Hinh"); [set_solver-..|]. wp_seq.
         iIntros "#Htok !>". wp_seq. iMod ("HκsI" with "Htok") as ">Hκs".
         iApply ("Hk" with "Htl HL Hκs"). rewrite tctx_hasty_val. done.
       + rewrite /tctx_interp vec_to_list_map !zip_with_fmap_r
